Cslib/Logics/Propositional/Semantics/Kripke.lean
@@ -1,0 +1,91 @@
+/-
+Copyright (c) 2025 Thomas Waring. All rights reserved.
+Released under Apache 2.0 license as described in the file LICENSE.
+Authors: Thomas Waring
+-/
+module
+
+public import Cslib.Logics.Propositional.NaturalDeduction.Basic
+public import Mathlib.Order.Heyting.Basic
+
+@[expose] public section
+
+namespace Cslib.Logic.PL
+
+open Proposition Theory InferenceSystem DerivableIn
+
+variable {Atom : Type u} {T : Theory Atom}
+
+structure KripkeModel (Atom Worlds : Type*) [PartialOrder Worlds] where
+  Forces' : Worlds → Atom → Prop
+  forces'_monotone : Monotone Forces'
+
+variable {Worlds : Type*} [PartialOrder Worlds] {C : KripkeModel Atom Worlds}
+
+def KripkeModel.Forces (C : KripkeModel Atom Worlds) (c : Worlds) : Proposition Atom → Prop
+  | atom x => C.Forces' c x
+  | Proposition.and A B => C.Forces c A ∧ C.Forces c B
+  | Proposition.or A B => C.Forces c A ∨ C.Forces c B
+  | impl A B => ∀ c' : Worlds, c ≤ c' → C.Forces c' A → C.Forces c' B
+
+scoped notation c " ⊨[" C "] " A => KripkeModel.Forces C c A
+
+lemma KripkeModel.forces_monotone {c c' : Worlds} (h : c ≤ c') (A : Proposition Atom) (hc : c ⊨[C] A) :
+    c' ⊨[C] A := by
+  induction A with
+  | atom x => exact C.forces'_monotone h x hc
+  | and A B aih bih => exact ⟨aih hc.1, bih hc.2⟩
+  | or A B aih bih =>
+    cases hc with
+    | inl hA => exact Or.inl <| aih hA
+    | inr hB => exact Or.inr <| bih hB
+  | impl A B aih bih =>
+    intro c'' h' hA
+    exact hc c'' (h.trans h') hA
+
+-- def Theory.Derivation.size {T : Theory Atom} [DecidableEq Atom] {Γ : Ctx Atom}
+--     {B : Proposition Atom} (D : T.Derivation (Γ ⊢ B)) : ℕ :=
+--   match D with
+--   | ax _ | ass _ => 1
+--   | conjI D D' | implE D D' => D.size + D'.size + 1
+--   | conjE₁ D | conjE₂ D | disjI₁ D | disjI₂ D | implI _ D => D.size + 1
+--   | disjE D D' D'' => D.size + D'.size + D''.size + 1
+--   termination_by sizeOf D
+
+theorem Theory.Derivation.forces [DecidableEq Atom] {Γ : Ctx Atom} {B : Proposition Atom}
+    {c : Worlds} (hT : ∀ A ∈ T, c ⊨[C] A) (D : T.Derivation Γ B) (hΓ : ∀ A ∈ Γ, c ⊨[C] A) :
+    c ⊨[C] B := by
+  induction D generalizing c with
+  | ax hB => exact hT _ hB
+  | ass hB => exact hΓ _ hB
+  | conjI DA DB aih bih => exact ⟨aih hT hΓ, bih hT hΓ⟩
+  | conjE₁ D ih => exact (ih hT hΓ).1
+  | conjE₂ D ih => exact (ih hT hΓ).2
+  | disjI₁ D ih => exact Or.inl <| ih hT hΓ
+  | disjI₂ D ih => exact Or.inr <| ih hT hΓ
+  | disjE D DA DB ih aih bih =>
+    cases ih hT hΓ with
+    | inl hA =>
+      apply aih hT
+      simp_rw [Finset.mem_insert]
+      rintro A' (rfl | hA')
+      · exact hA
+      · exact hΓ A' hA'
+    | inr hB =>
+      apply bih hT
+      simp_rw [Finset.mem_insert]
+      rintro A' (rfl | hA')
+      · exact hB
+      · exact hΓ A' hA'
+  | implI Γ D ih =>
+    intro c' hc hA
+    apply ih
+    · intro _ h
+      exact (C.forces_monotone hc) _ (hT _ h)
+    · simp_rw [Finset.mem_insert]
+      rintro A' (rfl | hA')
+      · exact hA
+      · exact (C.forces_monotone hc) A' (hΓ A' hA')
+  | implE D D' ih ih' => exact ih hT hΓ _ (le_refl c) <| ih' hT hΓ
+
+end Cslib.Logic.PL
